src/asn1/ASN1.Spec.BOOLEAN.fsti
@@ -34,14 +34,16 @@ val parse_asn1_boolean
 val parse_asn1_boolean_unfold
   (input: bytes)
 : Lemma (
-  parser_kind_prop parse_asn1_boolean_kind parse_asn1_boolean /\
   parse parse_asn1_boolean input ==
  (match parse parse_u8 input with
   | Some (x, consumed) -> if filter_asn1_boolean x then
                           ( Some (synth_asn1_boolean x, consumed) )
                           else
                           ( None )
-  | None -> None))
+  | None -> None) /\
+ (Some? (parse parse_asn1_boolean input) ==>
+   Seq.length input > 0 /\
+   parse parse_u8 input == Some (input.[0], 1)))
 
 val serialize_asn1_boolean
 : serializer parse_asn1_boolean
@@ -49,6 +51,9 @@ val serialize_asn1_boolean
 val serialize_asn1_boolean_unfold
   (b: datatype_of_asn1_type BOOLEAN)
 : Lemma (
+  serialize serialize_u8 (synth_asn1_boolean_inverse b)
+  `Seq.equal`
+  Seq.create 1 (synth_asn1_boolean_inverse b) /\
   serialize serialize_asn1_boolean b
   `Seq.equal`
   serialize serialize_u8 (synth_asn1_boolean_inverse b))
@@ -68,11 +73,12 @@ val synth_asn1_boolean_TLV_inverse
 
 let parse_asn1_boolean_TLV_kind
 : parser_kind
-= parse_asn1_tag_kind
-  `and_then_kind`
-  parse_asn1_length_kind_of_type BOOLEAN
-  `and_then_kind`
-  parse_asn1_boolean_kind
+= strong_parser_kind 3 3 None
+// = parse_asn1_tag_kind
+//   `and_then_kind`
+//   parse_asn1_length_kind_of_type BOOLEAN
+//   `and_then_kind`
+//   parse_asn1_boolean_kind
 
 let parse_asn1_boolean_TLV
 : parser parse_asn1_boolean_TLV_kind (datatype_of_asn1_type BOOLEAN)
@@ -88,17 +94,20 @@ val parse_asn1_boolean_TLV_unfold
   (input_TLV: bytes)
 : Lemma (
   parse parse_asn1_boolean_TLV input_TLV ==
- (match parse (parse_the_asn1_tag BOOLEAN) input_TLV with
+ (parser_kind_prop_equiv parse_asn1_tag_kind (parse_the_asn1_tag BOOLEAN);
+  match parse (parse_the_asn1_tag BOOLEAN) input_TLV with
   | None -> None
-  | Some (BOOLEAN, consumed_T) ->
-    (let input_LV = Seq.slice input_TLV consumed_T (Seq.length input_TLV) in
+  | Some (BOOLEAN, 1) ->
+    (parser_kind_prop_equiv (parse_asn1_length_kind_of_type BOOLEAN) (parse_asn1_length_of_type BOOLEAN);
+     let input_LV = Seq.slice input_TLV 1 (Seq.length input_TLV) in
      match parse (parse_asn1_length_of_type BOOLEAN) input_LV with
      | None -> None
-     | Some (1ul, consumed_L) ->
-       (let input_V = Seq.slice input_LV consumed_L (Seq.length input_LV) in
+     | Some (1ul, 1) ->
+       (parser_kind_prop_equiv parse_asn1_boolean_kind parse_asn1_boolean;
+        let input_V = Seq.slice input_LV 1 (Seq.length input_LV) in
         match parse parse_asn1_boolean input_V with
         | None -> None
-        | Some (value, consumed_V) -> Some (value, (consumed_T + consumed_L + consumed_V <: consumed_length input_TLV)))))
+        | Some (value, 1) -> Some (value, (1 + 1 + 1 <: consumed_length input_TLV)))))
 )
 
 let serialize_asn1_boolean_TLV
